src/Std/Tactic/BVDecide/LRAT/Internal/Convert.lean
@@ -61,7 +61,7 @@ theorem CNF.Clause.mem_lrat_of_mem (clause : CNF.Clause (PosFin n)) (h1 : l ∈ 
   | nil => cases h1
   | cons hd tl ih =>
     unfold DefaultClause.ofArray at h2
-    rw [← Array.foldr_toList, List.toArray_toList] at h2
+    rw [← Array.foldr_toList, Array.toArray_toList] at h2
     dsimp only [List.foldr] at h2
     split at h2
     · cases h2
@@ -77,7 +77,7 @@ theorem CNF.Clause.mem_lrat_of_mem (clause : CNF.Clause (PosFin n)) (h1 : l ∈ 
             · assumption
             · next heq _ _ =>
               unfold DefaultClause.ofArray
-              rw [← Array.foldr_toList, List.toArray_toList]
+              rw [← Array.foldr_toList, Array.toArray_toList]
               exact heq
         · cases h1
           · simp only [← Option.some.inj h2]
@@ -89,7 +89,7 @@ theorem CNF.Clause.mem_lrat_of_mem (clause : CNF.Clause (PosFin n)) (h1 : l ∈ 
             apply ih
             assumption
             unfold DefaultClause.ofArray
-            rw [← Array.foldr_toList, List.toArray_toList]
+            rw [← Array.foldr_toList, Array.toArray_toList]
             exact heq
 
 theorem CNF.Clause.convertLRAT_sat_of_sat (clause : CNF.Clause (PosFin n))
@@ -155,7 +155,7 @@ theorem CNF.unsat_of_convertLRAT_unsat (cnf : CNF Nat) :
   simp only [Formula.formulaEntails_def, List.all_eq_true, decide_eq_true_eq]
   intro lratClause hlclause
   simp only [Formula.toList, DefaultFormula.toList, DefaultFormula.ofArray,
-    CNF.convertLRAT', Array.size_toArray, List.length_map, Array.toList_toArray,
+    CNF.convertLRAT', List.size_toArray, List.length_map, List.toList_toArray,
     List.map_nil, List.append_nil, List.mem_filterMap, List.mem_map, id_eq, exists_eq_right] at hlclause
   rcases hlclause with ⟨reflectClause, ⟨hrclause1, hrclause2⟩⟩
   simp only [CNF.eval, List.all_eq_true] at h2
