src/Std/Tactic/BVDecide/LRAT/Internal/Formula/RupAddResult.lean
@@ -392,7 +392,7 @@ theorem insertUnitInvariant_insertRupUnits {n : Nat} (f : DefaultFormula n) (f_r
     simp only [Fin.getElem_fin, ne_eq, true_and, Bool.not_eq_true, exists_and_right]
     apply Or.inl
     intro j
-    simp only [f_readyForRupAdd.1, Array.size_toArray, List.length_nil] at j
+    simp only [f_readyForRupAdd.1, List.size_toArray, List.length_nil] at j
     exact Fin.elim0 j
   exact insertUnitInvariant_insertUnit_fold f.assignments hsize f.rupUnits f.assignments hsize false units h0
 
@@ -1114,11 +1114,11 @@ theorem nodup_derivedLits {n : Nat} (f : DefaultFormula n)
     simp [li, Array.getElem_mem]
   have i_in_bounds : i.1 < derivedLits.length := by
     have i_property := i.2
-    simp only [derivedLits_arr_def, Array.size_toArray] at i_property
+    simp only [derivedLits_arr_def, List.size_toArray] at i_property
     exact i_property
   have j_in_bounds : j.1 < derivedLits.length := by
     have j_property := j.2
-    simp only [derivedLits_arr_def, Array.size_toArray] at j_property
+    simp only [derivedLits_arr_def, List.size_toArray] at j_property
     exact j_property
   rcases derivedLits_satisfies_invariant ⟨li.1.1, li.1.2.2⟩ with ⟨_, h2⟩ | ⟨k, _, _, _, h3⟩ |
     ⟨k1, k2, _, _, k1_eq_true, k2_eq_false, _, _, h3⟩
@@ -1215,7 +1215,7 @@ theorem restoreAssignments_performRupCheck_base_case {n : Nat} (f : DefaultFormu
       exact h2 derivedLits_arr[j] idx_in_list
   · apply Or.inr ∘ Or.inl
     have j_lt_derivedLits_arr_size : j.1 < derivedLits_arr.size := by
-      simp only [derivedLits_arr_def, Array.size_toArray]
+      simp only [derivedLits_arr_def, List.size_toArray]
       exact j.2
     have i_gt_zero : i.1 > 0 := by rw [← j_eq_i]; exact (List.get derivedLits j).1.2.1
     refine ⟨⟨j.1, j_lt_derivedLits_arr_size⟩, List.get derivedLits j |>.2, i_gt_zero, ?_⟩
@@ -1228,7 +1228,7 @@ theorem restoreAssignments_performRupCheck_base_case {n : Nat} (f : DefaultFormu
         intro k _ k_ne_j
         have k_in_bounds : k < derivedLits.length := by
           have k_property := k.2
-          simp only [derivedLits_arr_def, Array.size_toArray] at k_property
+          simp only [derivedLits_arr_def, List.size_toArray] at k_property
           exact k_property
         have k_ne_j : ⟨k.1, k_in_bounds⟩ ≠ j := by
           apply Fin.ne_of_val_ne
@@ -1238,10 +1238,10 @@ theorem restoreAssignments_performRupCheck_base_case {n : Nat} (f : DefaultFormu
         exact h3 ⟨k.1, k_in_bounds⟩ k_ne_j
   · apply Or.inr ∘ Or.inr
     have j1_lt_derivedLits_arr_size : j1.1 < derivedLits_arr.size := by
-      simp only [derivedLits_arr_def, Array.size_toArray]
+      simp only [derivedLits_arr_def, List.size_toArray]
       exact j1.2
     have j2_lt_derivedLits_arr_size : j2.1 < derivedLits_arr.size := by
-      simp only [derivedLits_arr_def, Array.size_toArray]
+      simp only [derivedLits_arr_def, List.size_toArray]
       exact j2.2
     have i_gt_zero : i.1 > 0 := by rw [← j1_eq_i]; exact (List.get derivedLits j1).1.2.1
     refine ⟨⟨j1.1, j1_lt_derivedLits_arr_size⟩,
@@ -1259,7 +1259,7 @@ theorem restoreAssignments_performRupCheck_base_case {n : Nat} (f : DefaultFormu
         intro k _ k_ne_j1 k_ne_j2
         have k_in_bounds : k < derivedLits.length := by
           have k_property := k.2
-          simp only [derivedLits_arr_def, Array.size_toArray] at k_property
+          simp only [derivedLits_arr_def, List.size_toArray] at k_property
           exact k_property
         have k_ne_j1 : ⟨k.1, k_in_bounds⟩ ≠ j1 := by
           apply Fin.ne_of_val_ne
